protocol spec for appendEntriesRequest

ironfleet/src/Dafny/Distributed/Protocol/Raft/Server.i.dfy
@@ -6,6 +6,7 @@
 include "../../Common/Framework/Environment.s.dfy"
 include "../../Services/Raft/AppStateMachine.s.dfy"
 include "../Common/UpperBound.s.dfy"
+include "../Common/Utils.s.dfy"
 include "Config.i.dfy"
 include "Types.i.dfy"
 
@@ -14,6 +15,7 @@ module Raft__Server_i {
 import opened Environment_s
 import opened AppStateMachine_s
 import opened Common__UpperBound_s
+import opened Common__Utils_s
 import opened Raft__Config_i
 import opened Raft__Types_i
 
@@ -24,6 +26,7 @@ datatype RaftServer = RaftServer(
   next_heartbeat_time:int,
   next_election_time:int,
   // persistent state
+  current_leader:int,
   current_term:int,
   voted_for:int,
   log:seq<LogEntry>,
@@ -67,14 +70,31 @@ function SpontaneousClock(ios:seq<RaftIo>) : ClockReading
 ////////////////////////////////////////////////
 // Utils
 ////////////////////////////////////////////////
-function RaftPrevLogIndex(s:RaftServer) : int
+function RaftLastLogIndex(s:RaftServer) : int
 {
   if s.log == [] then 0 else s.log[|s.log|-1].index
 }
 
-function RaftPrevLogTerm(s:RaftServer) : int
+function RaftLastLogTerm(s:RaftServer) : int
 {
   if s.log == [] then 0 else s.log[|s.log|-1].term
+}
+
+function RaftGetLogEntry(s:RaftServer, index:int) : LogEntry
+  requires 0 < index <= |s.log|
+{
+  s.log[index-1]
+}
+
+function {:opaque} ExtractSentPacketsFromIos(ios:seq<RaftIo>) : seq<RaftPacket>
+  ensures forall p :: p in ExtractSentPacketsFromIos(ios) <==> LIoOpSend(p) in ios
+{
+  if |ios| == 0 then
+    []
+  else if ios[0].LIoOpSend? then
+    [ios[0].s] + ExtractSentPacketsFromIos(ios[1..])
+  else
+    ExtractSentPacketsFromIos(ios[1..])
 }
 
 predicate RaftBroadcastToEveryone(config:RaftConfig, myidx:int, m:RaftMessage, sent_packets:seq<RaftPacket>)
@@ -88,60 +108,131 @@ predicate RaftBroadcastToEveryone(config:RaftConfig, myidx:int, m:RaftMessage, s
 ////////////////////////////////////////////////
 // Handle received packets
 ////////////////////////////////////////////////
-predicate RaftServerNextHandleRequestVote(s:RaftServer, s':RaftServer, ios:seq<RaftIo>)
+predicate RaftServerMaybeStepDown(s:RaftServer, s':RaftServer, term:int)
 {
-  true
+  if s.current_term < term then
+    && s'.role == Follower
+    && s'.voted_for == -1
+    && s'.current_term == term
+  else
+    s'.role == s.role
+    && s'.voted_for == s.voted_for
+    && s'.current_term == s.current_term
 }
 
-predicate RaftServerNextHandleRequestVoteReply(s:RaftServer, s':RaftServer, ios:seq<RaftIo>)
+predicate RaftServerMaybeResetElectionTimeout(s:RaftServer, s':RaftServer, clock:int, msg:RaftMessage)
+  requires msg.RaftMessage_AppendEntries?
 {
-  true
+  var global_config := s.config.global_config;
+  msg.leader_id == s.current_leader ==> exists election_timeout :: (
+    && global_config.min_election_timeout <= election_timeout <= global_config.max_election_timeout
+    && s' == s.(next_election_time := UpperBoundedAddition(clock, election_timeout, global_config.max_integer_value))
+  )
 }
 
-predicate RaftServerNextHandleAppendEntries(s:RaftServer, s':RaftServer, ios:seq<RaftIo>)
+predicate RaftServerNextHandleAppendEntries(s:RaftServer, s':RaftServer, received_packet: RaftPacket, clock:int, sent_packages:seq<RaftPacket>)
+  requires received_packet.msg.RaftMessage_AppendEntries?
 {
-  true
+  var received_msg := received_packet.msg;
+  // maybe step down
+  && RaftServerMaybeStepDown(s, s', received_packet.msg.term)
+  // handle the entries
+  && received_msg.prev_log_index >= 0
+  && forall entry :: entry in received_packet.msg.entries ==> LogEntryValid(entry)
+  // No matter when receiving this, a follower should reset its election timeout
+  && RaftServerMaybeResetElectionTimeout(s, s', clock, received_msg)
+  && (
+    var entries := received_packet.msg.entries;
+    if (
+      || received_msg.prev_log_index == 0
+      || (&& received_msg.prev_log_index <= |s.log| 
+          && RaftGetLogEntry(s, received_msg.prev_log_index).term == received_msg.prev_log_term
+          )
+    ) then
+      // entries should be appended
+      && |s'.log| == |s.log| + |entries|
+      && forall entry :: entry in entries ==> 0 < entry.index <= |s'.log| && RaftGetLogEntry(s', entry.index) == entry
+      && |sent_packages| == 1
+      && var sent_msg := sent_packages[0].msg;
+        && sent_msg.RaftMessage_AppendEntriesReply?
+        && sent_msg.term == s'.current_term
+        && sent_msg.success == true
+        && sent_msg.match_index == RaftLastLogIndex(s')
+    else
+      // or discarded
+      && s'.log == s.log
+      && |sent_packages| == 1
+      && var sent_msg := sent_packages[0].msg;
+        && sent_msg.RaftMessage_AppendEntriesReply?
+        && sent_msg.term == s'.current_term
+        && sent_msg.success == false
+  )
 }
 
-predicate RaftServerNextHandleAppendEntriesReply(s:RaftServer, s':RaftServer, ios:seq<RaftIo>)
+predicate RaftServerNextHandleAppendEntriesReply(s:RaftServer, s':RaftServer, received_packet: RaftPacket, sent_packages:seq<RaftPacket>)
+  requires received_packet.msg.RaftMessage_AppendEntriesReply?
 {
-  true
+  // maybe step down
+  && RaftServerMaybeStepDown(s, s', received_packet.msg.term)
+}
+
+predicate RaftServerNextHandleRequestVote(s:RaftServer, s':RaftServer, received_packet: RaftPacket, sent_packages:seq<RaftPacket>)
+  requires received_packet.msg.RaftMessage_RequestVote?
+{
+  // maybe step down
+  && RaftServerMaybeStepDown(s, s', received_packet.msg.term)
+}
+
+predicate RaftServerNextHandleRequestVoteReply(s:RaftServer, s':RaftServer, received_packet: RaftPacket, sent_packages:seq<RaftPacket>)
+  requires received_packet.msg.RaftMessage_RequestVoteReply?
+{
+  // maybe step down
+  && RaftServerMaybeStepDown(s, s', received_packet.msg.term)
+}
+
+predicate LReplicaNextReadClockAndProcessPacket(s:RaftServer, s':RaftServer, ios:seq<RaftIo>)
+  requires |ios| >= 1
+  requires ios[0].LIoOpReceive?
+  requires ios[0].r.msg.RaftMessage_AppendEntries?
+{
+  && |ios| > 1
+  && ios[1].LIoOpReadClock?
+  && (forall io :: io in ios[2..] ==> io.LIoOpSend?)
+  && forall entry :: entry in ios[0].r.msg.entries ==> LogEntryValid(entry)
+  && RaftServerNextHandleAppendEntries(s, s', ios[0].r, ios[1].t, ExtractSentPacketsFromIos(ios))
+}
+
+predicate RaftServerNextProcessPacketWithoutReadingClock(s:RaftServer, s':RaftServer, ios:seq<RaftIo>)
+  requires |ios| >= 1
+  requires ios[0].LIoOpReceive?
+  requires !ios[0].r.msg.RaftMessage_AppendEntries?
+{
+  && forall io :: io in ios[1..] ==> io.LIoOpSend?
+  && var sent_packets := ExtractSentPacketsFromIos(ios);
+    match ios[0].r.msg
+      case RaftMessage_RequestVote(_,_,_,_) => RaftServerNextHandleRequestVote(s, s', ios[0].r, sent_packets)
+      case RaftMessage_RequestVoteReply(_,_) => RaftServerNextHandleRequestVoteReply(s, s', ios[0].r, sent_packets)
+      case RaftMessage_AppendEntriesReply(_,_,_) => RaftServerNextHandleAppendEntriesReply(s, s', ios[0].r, sent_packets)
 }
 
 predicate RaftServerNextProcessPacket(s:RaftServer, s':RaftServer, ios:seq<RaftIo>)
 {
   && |ios| >= 1
   && if ios[0].LIoOpTimeoutReceive? then
-      s' == s && |ios| == 1 // TODO: why?
+      s' == s && |ios| == 1 // TODO: why? (maybe due to implmentation)
     else
       (
         && ios[0].LIoOpReceive?
-        && if ios[0].r.msg.RaftMessage_RequestVote? then
-            RaftServerNextHandleRequestVote(s, s', ios)
-          else if ios[0].r.msg.RaftMessage_RequestVoteReply? then
-            RaftServerNextHandleRequestVoteReply(s, s', ios)
-          else if ios[0].r.msg.RaftMessage_AppendEntries? then
-            // Note: this is the only one that may requires a election timeout reset
-            RaftServerNextHandleAppendEntries(s, s', ios)
+        && if ios[0].r.msg.RaftMessage_AppendEntries? then
+            LReplicaNextReadClockAndProcessPacket(s, s', ios)
           else
-            ios[0].r.msg.RaftMessage_AppendEntriesReply? && RaftServerNextHandleAppendEntriesReply(s, s', ios)
+            RaftServerNextProcessPacketWithoutReadingClock(s, s', ios)
       )
 }
 
 ////////////////////////////////////////////////
 // Handle other events
 ////////////////////////////////////////////////
-function {:opaque} ExtractSentPacketsFromIos(ios:seq<RaftIo>) : seq<RaftPacket>
-  ensures forall p :: p in ExtractSentPacketsFromIos(ios) <==> LIoOpSend(p) in ios
-{
-  if |ios| == 0 then
-    []
-  else if ios[0].LIoOpSend? then
-    [ios[0].s] + ExtractSentPacketsFromIos(ios[1..])
-  else
-    ExtractSentPacketsFromIos(ios[1..])
-}
-
 predicate RaftServerNextReadClockMaybeSendHeartbeat(s:RaftServer, s':RaftServer, clock:ClockReading, sent_packets:seq<RaftPacket>)
 {
   && s.role.Leader?
@@ -154,7 +245,7 @@ predicate RaftServerNextReadClockMaybeSendHeartbeat(s:RaftServer, s':RaftServer,
         s.config.global_config, s.config.server_id, 
         RaftMessage_AppendEntries(
           s.current_term, s.config.server_id, 
-          RaftPrevLogIndex(s), RaftPrevLogTerm(s), 
+          RaftLastLogIndex(s), RaftLastLogTerm(s), 
           [], s.commit_index),
         sent_packets)
       && s' == s.(next_heartbeat_time := s'.next_heartbeat_time)
@@ -173,7 +264,7 @@ predicate RaftServerNextReadClockMaybeStartElection(s:RaftServer, s':RaftServer,
         s.config.global_config, s.config.server_id, 
         RaftMessage_RequestVote(
           s.current_term, s.config.server_id, 
-          RaftPrevLogIndex(s), RaftPrevLogTerm(s)),
+          RaftLastLogIndex(s), RaftLastLogTerm(s)),
         sent_packets)
       && s' == s.(next_election_time := s'.next_election_time)
   )
@@ -203,7 +294,7 @@ predicate RaftServerNoReceiveNext(s:RaftServer, nextActionIndex:int, s':RaftServ
 
 function RaftServerNumActions() : int
 {
-  10
+  2
 }
 
 }
