ironfleet/src/Dafny/Distributed/Protocol/Raft/Types.i.dfy
@@ -12,16 +12,21 @@ type RaftEnvironment = LEnvironment<EndPoint, RaftMessage>
 type RaftPacket = LPacket<EndPoint, RaftMessage>
 type RaftIo = LIoOp<EndPoint, RaftMessage>
 
+datatype LogEntry = LogEntry(term:int, index:int, req:AppRequest)
+
+predicate LogEntryValid(entry:LogEntry) {
+  && entry.term > 0 && entry.index > 0
+}
+
 datatype RaftMessage =
     RaftMessage_RequestVote(term:int, candidate_id:int, last_log_index:int, last_log_term:int)
   | RaftMessage_RequestVoteReply(term:int, vote_granted:bool)
-  | RaftMessage_AppendEntries(term:int, leader_id:int, prev_log_index:int, prev_log_term:int, entries:seq<AppRequest>, leader_commit:int)
-  | RaftMessage_AppendEntriesReply(term:int, success:bool)
+  | RaftMessage_AppendEntries(term:int, leader_id:int, prev_log_index:int, prev_log_term:int, entries:seq<LogEntry>, leader_commit:int)
+  | RaftMessage_AppendEntriesReply(term:int, success:bool, match_index:int)
 
 datatype RaftRole = Follower | Candidate | Leader
 
 datatype ClockReading = ClockReading(t:int)
 
-datatype LogEntry = LogEntry(term:int, index:int, req:AppRequest)
 
 }
