ironfleet/src/Dafny/Distributed/Protocol/Common/Utils.s.dfy
@@ -1,0 +1,7 @@
+module Common__Utils_s {
+
+function max(a:int, b:int):int
+{
+  if a >= b then a else b
+}
+}
